dist/gcc-compatible/lib/Hacl_Bignum_bindings.ml
@@ -2,31 +2,18 @@ open Ctypes
 module Bindings(F:Cstubs.FOREIGN) =
   struct
     open F
-    let hacl_Bignum_Multiplication_mul_carry_add_u64_st =
-      foreign "Hacl_Bignum_Multiplication_mul_carry_add_u64_st"
-        (uint64_t @->
-           (uint64_t @->
-              (uint64_t @-> ((ptr uint64_t) @-> (returning uint64_t)))))
-    let hacl_Bignum_Karatsuba_bn_karatsuba_mul_ =
-      foreign "Hacl_Bignum_Karatsuba_bn_karatsuba_mul_"
+    let hacl_Bignum_Karatsuba_bn_karatsuba_mul_uint64 =
+      foreign "Hacl_Bignum_Karatsuba_bn_karatsuba_mul_uint64"
         (uint32_t @->
            ((ptr uint64_t) @->
               ((ptr uint64_t) @->
                  ((ptr uint64_t) @-> ((ptr uint64_t) @-> (returning void))))))
-    let hacl_Bignum_Karatsuba_bn_karatsuba_sqr_ =
-      foreign "Hacl_Bignum_Karatsuba_bn_karatsuba_sqr_"
+    let hacl_Bignum_Karatsuba_bn_karatsuba_sqr_uint64 =
+      foreign "Hacl_Bignum_Karatsuba_bn_karatsuba_sqr_uint64"
         (uint32_t @->
            ((ptr uint64_t) @->
               ((ptr uint64_t) @-> ((ptr uint64_t) @-> (returning void)))))
-    let hacl_Bignum_bn_get_ith_bit =
-      foreign "Hacl_Bignum_bn_get_ith_bit"
-        (uint32_t @->
-           ((ptr uint64_t) @-> (uint32_t @-> (returning uint64_t))))
-    let hacl_Bignum_bn_lt_mask =
-      foreign "Hacl_Bignum_bn_lt_mask"
-        (uint32_t @->
-           ((ptr uint64_t) @-> ((ptr uint64_t) @-> (returning uint64_t))))
-    let hacl_Bignum_ModInv64_mod_inv_u64 =
-      foreign "Hacl_Bignum_ModInv64_mod_inv_u64"
+    let hacl_Bignum_ModInvLimb_mod_inv_uint64 =
+      foreign "Hacl_Bignum_ModInvLimb_mod_inv_uint64"
         (uint64_t @-> (returning uint64_t))
   end
