dist/gcc-compatible/lib/Hacl_RSAPSS_bindings.ml
@@ -6,26 +6,29 @@ module Bindings(F:Cstubs.FOREIGN) =
     open Hacl_Spec_applied
     let hacl_RSAPSS_rsapss_sign =
       foreign "Hacl_RSAPSS_rsapss_sign"
-        (spec_Hash_Definitions_hash_alg @->
-           (uint32_t @->
+        (uint32_t @->
+           (spec_Hash_Definitions_hash_alg @->
+              (uint32_t @->
+                 (uint32_t @->
+                    (uint32_t @->
+                       ((ptr uint64_t) @->
+                          (uint32_t @->
+                             (ocaml_bytes @->
+                                (uint32_t @->
+                                   (ocaml_bytes @->
+                                      (ocaml_bytes @-> (returning bool))))))))))))
+    let hacl_RSAPSS_rsapss_verify =
+      foreign "Hacl_RSAPSS_rsapss_verify"
+        (uint32_t @->
+           (spec_Hash_Definitions_hash_alg @->
               (uint32_t @->
                  (uint32_t @->
                     ((ptr uint64_t) @->
                        (uint32_t @->
-                          (ocaml_bytes @->
-                             (uint32_t @->
-                                (ocaml_bytes @->
+                          (uint32_t @->
+                             (ocaml_bytes @->
+                                (uint32_t @->
                                    (ocaml_bytes @-> (returning bool)))))))))))
-    let hacl_RSAPSS_rsapss_verify =
-      foreign "Hacl_RSAPSS_rsapss_verify"
-        (spec_Hash_Definitions_hash_alg @->
-           (uint32_t @->
-              (uint32_t @->
-                 ((ptr uint64_t) @->
-                    (uint32_t @->
-                       (uint32_t @->
-                          (ocaml_bytes @->
-                             (uint32_t @-> (ocaml_bytes @-> (returning bool))))))))))
     let hacl_RSAPSS_new_rsapss_load_pkey =
       foreign "Hacl_RSAPSS_new_rsapss_load_pkey"
         (uint32_t @->
@@ -41,28 +44,30 @@ module Bindings(F:Cstubs.FOREIGN) =
                        (ocaml_bytes @-> (returning (ptr uint64_t))))))))
     let hacl_RSAPSS_rsapss_skey_sign =
       foreign "Hacl_RSAPSS_rsapss_skey_sign"
-        (spec_Hash_Definitions_hash_alg @->
-           (uint32_t @->
+        (uint32_t @->
+           (spec_Hash_Definitions_hash_alg @->
+              (uint32_t @->
+                 (uint32_t @->
+                    (uint32_t @->
+                       (ocaml_bytes @->
+                          (ocaml_bytes @->
+                             (ocaml_bytes @->
+                                (uint32_t @->
+                                   (ocaml_bytes @->
+                                      (uint32_t @->
+                                         (ocaml_bytes @->
+                                            (ocaml_bytes @-> (returning bool))))))))))))))
+    let hacl_RSAPSS_rsapss_pkey_verify =
+      foreign "Hacl_RSAPSS_rsapss_pkey_verify"
+        (uint32_t @->
+           (spec_Hash_Definitions_hash_alg @->
               (uint32_t @->
                  (uint32_t @->
                     (ocaml_bytes @->
                        (ocaml_bytes @->
-                          (ocaml_bytes @->
+                          (uint32_t @->
                              (uint32_t @->
                                 (ocaml_bytes @->
                                    (uint32_t @->
-                                      (ocaml_bytes @->
-                                         (ocaml_bytes @-> (returning bool)))))))))))))
-    let hacl_RSAPSS_rsapss_pkey_verify =
-      foreign "Hacl_RSAPSS_rsapss_pkey_verify"
-        (spec_Hash_Definitions_hash_alg @->
-           (uint32_t @->
-              (uint32_t @->
-                 (ocaml_bytes @->
-                    (ocaml_bytes @->
-                       (uint32_t @->
-                          (uint32_t @->
-                             (ocaml_bytes @->
-                                (uint32_t @->
-                                   (ocaml_bytes @-> (returning bool)))))))))))
+                                      (ocaml_bytes @-> (returning bool))))))))))))
   end
